%! Author = anton
%! Date = 7/13/24

% Preamble
\documentclass[9pt]{article}

% Packages
\usepackage[a4paper, total={6.75in, 11in}, left=15mm, top=15mm]{geometry}
\usepackage{amsmath}
\usepackage{amssymb}
\newtheorem{theorem}{Theorem}[section]
\newtheorem{proof}{Proof}
\renewenvironment{proof}{{\bf \emph{Proof.} }}{\hfill $\Box$ \\}

\numberwithin{equation}{section}
% Document
\begin{document}

\title{\sc Theory behind steady camera filter}
\author{Anton Morzhakov}
\maketitle

\section{Fourier series}\label{sec:theory-behind-fourier-series}
\subsection{Basic Form}\label{subsec:basic-form}
Formally consider function, represented by series:
\begin{equation}\label{eq:equation}
    f(t) \sim a_0 + \sum_{n=1}^{\infty} a_n \sin (n \omega_0 t + \phi_n),
\end{equation}
where $a_0$ -- constant, $a_n$ and $\phi_n$, $n \geq 1$ are amplitudes and phase shifts respectively,
$\omega_0$ is the base frequency, e.g. $\omega_0 = \frac{2\pi}{T}$, $T$  is a period.
If we make substitution
\[
    x = \omega_0 t  = \frac{2\pi t}{T},
\]
then
\begin{equation}\label{eq:equation2}
    f(x) \sim a_0 + \sum_{n=1}^{\infty} a_n \sin (n x + \phi_n).
\end{equation}
Using trigonometric formula
\[
    \sin (\alpha +  \beta)  = \sin \alpha \cos \beta + \cos \alpha \sin \beta
\]
we get representation
\begin{equation}\label{eq:equation3}
    f(x) \sim c_{0, 0} + \sum_{n=1}^{\infty} \left( c_{n, 1} \cos nx + c_{n, 2} \sin nx \right).
\end{equation}
Note that now amplitude $a_n = \|(c_{n, 1}, c_{n, 2})\|_2$ and phase $\phi_n = \mathrm{atan2} (c_{n, 2}, c_{n, 1})$,
$a_0 = c_{0, 0}$.

\subsection{Complex Form}\label{subsec:complex-form}

If we substitute $\cos nx$ and $\sin nx$ with complex exponent
\begin{align*}
    \cos nx = & \frac{e^{nxi} + e^{-nxi}}{2}   \\
    \sin nx = & \frac{e^{nxi} - e^{-nxi}}{2i} = \frac{e^{-nxi} - e^{nxi}}{2} \\
\end{align*}
then we will get the following form of~\ref{eq:equation3}:
\begin{equation}\label{eq:equation4}
    f(x) \sim \frac{c_{0,0}}{2} + \sum_{n=1}^{\infty} \frac{c_{n, 1} - c_{n, 2}i}{2} e^{nxi} +
    \frac{c_{n, 1} + c_{n, 2}i}{2} e^{-nxi} = \allowbreak  \sum_{k=-\infty}^{+\infty} c_k e^{kxi},
\end{equation}
where
\begin{align}
    c_0 & = \frac{c_{0, 0}}{2} \\
    c_n &= \frac{c_{n,1} - c_{n,2}i}{2} \\
    c_{-n} &= \frac{c_{n,1} + c_{n,2}i}{2},
\end{align}
$c_{-n} = c_n^{\ast}$.
\subsection{Fourier Series Convergence Theorems}\label{subsec:fourier-series-convergence}

\section{Fourier Transform}\label{sec:fourier-transform}

\[
    \mathcal F \{ f(x) \}  = \hat f (\omega) = \langle f(x), e^{i \omega x} \rangle =
    \int_{\mathbb R} f(x) e^{-i \omega x} dx
\]

\begin{theorem}[Shift Theorem] \label{shift_theorem}
    Let \(f\) be a function, $a$ is a constant, then
    \[
        \mathcal F \{ f(x - a) \} =  e^{-i a \omega} \mathcal F \{ f(x) \}.
    \]
\end{theorem}

\begin{proof}
    \begin{multline}
        \mathcal F \{ f(x - a) \}  =  \int_{\mathbb R} f(x - a) e^{-i \omega x} dx =
        \int_{\mathbb R} f(x) e^{-i \omega (x + a)} dx = \allowbreak
        e^{-i a \omega} \int_{\mathbb R} f(x) e^{-i \omega x} dx = e^{-i a \omega} \mathcal F \{ f(x) \}
    \end{multline}
\end{proof}

\section{Phase Correlation}\label{sec:theory-behind-phase-correlation}

\section{Why do we need text and persons masking?}\label{sec:why-we-need-text-and-persond-masking?}

\end{document}